Seccompjit.v
@@ -1,61 +1,99 @@
+Require Import compcert.backend.RTL.
 Require Import compcert.common.AST.
 Require Import compcert.common.Errors.
-Require Import compcert.cfrontend.Clight.
-Require Import compcert.cfrontend.Cop.
-Require Import compcert.cfrontend.Ctypes.
 Require Import compcert.lib.Coqlib.
 Require Import compcert.lib.Integers.
 Require Import compcert.lib.Maps.
+Require Import Op.
 Require Import Seccomp.
 
 Parameter seccomp_memwords: Z.
 
-Definition id_a:   ident := 1%positive.
-Definition id_x:   ident := 2%positive.
-Definition id_mem: ident := 3%positive.
+Record state: Type := mkstate {
+  st_code: RTL.code;
+  st_ep: node;
+  st_map: ZMap.t node
+}.
 
-Definition u32: type := Tint I32 Unsigned noattr.
+Inductive state_incr: state -> state -> Prop :=
+  state_incr_intro:
+    forall (s1 s2: state),
+    Ple s1.(st_ep) s2.(st_ep) ->
+    (forall pc,
+      s1.(st_code)!pc = None \/ s2.(st_code)!pc = s1.(st_code)!pc) ->
+    state_incr s1 s2.
+
+Lemma state_incr_refl:
+  forall s, state_incr s s.
+Proof.
+  intros.
+  apply state_incr_intro.
+  apply Ple_refl.
+  intros; auto.
+Qed.
+
+Lemma state_incr_trans:
+  forall s1 s2 s3, state_incr s1 s2 -> state_incr s2 s3 -> state_incr s1 s3.
+Proof.
+  intros.
+  inv H; inv H0.
+  apply state_incr_intro.
+  apply Ple_trans with s2.(st_ep); assumption.
+
+  intros.
+  generalize (H2 pc) (H3 pc).
+  intuition congruence.
+Qed.
+
+Definition add_instr (instr: RTL.instruction) (st: state) : state :=
+  let n := Psucc st.(st_ep) in
+  mkstate (PTree.set n instr st.(st_code)) n st.(st_map).
+
+Definition add_map (pc: Z) (st: state) : state :=
+  mkstate st.(st_code) st.(st_ep) (ZMap.set pc st.(st_ep) st.(st_map)).
+
+Definition reg_a:   ident := 1%positive.
+Definition reg_x:   ident := 2%positive.
+Definition reg_mem: ident := 3%positive.
 
 Open Local Scope error_monad_scope.
 
-Definition transl_instr (instr: Seccomp.instruction) (n: label) : res statement :=
+Definition transl_instr (instr: Seccomp.instruction) (pc: Z) (st: state) : res state :=
   match instr with
   | Salu_add_k k =>
-    OK (Sset id_a (Ebinop Oadd (Etempvar id_a u32) (Econst_int k u32) u32))
-(*
-  | Sret_k k =>
-    OK (Sreturn (Some (Econst_int k type_int32s)))
-*)
+    OK (add_instr (Iop (Oaddimm k) (reg_a::nil) reg_a st.(st_ep)) st)
   | Sret_a =>
-    OK (Sreturn (Some (Ecast (Etempvar id_a u32) type_int32s)))
+    OK (add_instr (Ireturn (Some reg_a)) st)
   | _ => Error (msg "FIXME")
   end.
 
-Fixpoint transl_code (src: Seccomp.code) (n: label) : res statement :=
+Fixpoint transl_code (src: Seccomp.code) (pc: Z) (st: state) : res state :=
   match src with
-  | nil => OK Sskip
+  | nil => OK st
   | hd::tl =>
-    do bodytl <- transl_code tl (Psucc n);
-    do bodyhd <- transl_instr hd n;
-    OK (Slabel n (Ssequence bodyhd bodytl))
+    do st <- transl_code tl (Zsucc pc) st;
+    do st <- transl_instr hd pc st;
+    OK (add_map pc st)
   end.
 
-Definition transl_function (f: Seccomp.function) : res Clight.function :=
-  do body <- transl_code f xH;
-  let vars := (id_mem, Tarray u32 seccomp_memwords noattr)::nil in
-  let temps := (id_a, u32)::(id_x, u32)::nil in
+Definition transl_function (f: Seccomp.function) : res RTL.function :=
+  let st := mkstate (PTree.empty RTL.instruction) 1%positive (ZMap.init 1%positive) in
+  do st <- transl_code f 0 st;
+  let sig := mksignature nil (Some Tint) in
+  let stacksize := (Zmult seccomp_memwords 4) in
   (* FIXME: memset(mem, 0, sizeof(mem)) *)
-  let body := Ssequence (Sset id_x (Econst_int Int.zero u32)) body in
-  let body := Ssequence (Sset id_a (Econst_int Int.zero u32)) body in
-  OK (Clight.mkfunction type_int32s nil vars temps body).
-
-Definition transl_fundef (fd: Seccomp.fundef) : res Clight.fundef :=
-  match fd with
-  | AST.Internal f => do tf <- transl_function f; OK (Clight.Internal tf)
-  | _ => Error (msg "external function not allowed")
-  end.
+  let st := add_instr (Iop (Oaddrstack Int.zero) nil reg_mem st.(st_ep)) st in
+  let st := add_instr (Iop (Ointconst Int.zero) nil reg_x st.(st_ep)) st in
+  let st := add_instr (Iop (Ointconst Int.zero) nil reg_a st.(st_ep)) st in
+  OK (RTL.mkfunction sig nil stacksize st.(st_code) st.(st_ep)).
 
 Local Open Scope string_scope.
 
-Definition transl_program (p: Seccomp.program) : res Clight.program :=
+Definition transl_fundef (fd: fundef) :=
+  match fd with
+  | Internal f => do f' <- transl_function f; OK (Internal f')
+  | External ef => Error (msg "no external function allowed")
+  end.
+
+Definition transl_program (p: Seccomp.program) : res RTL.program :=
   transform_partial_program transl_fundef p.
