Seccompproof.v
@@ -1,5 +1,5 @@
-Require Import compcert.cfrontend.Clight.
-Require Import compcert.cfrontend.Ctypes.
+Require Import compcert.backend.RTL.
+Require Import compcert.backend.Registers.
 Require Import compcert.common.AST.
 Require Import compcert.common.Errors.
 Require Import compcert.common.Globalenvs.
@@ -7,13 +7,15 @@ Require Import compcert.common.Memory.
 Require Import compcert.common.Smallstep.
 Require Import compcert.common.Values.
 Require Import compcert.lib.Coqlib.
+Require Import compcert.lib.Integers.
+Require Import Op.
 Require Import Seccomp.
 Require Import Seccompjit.
 
 (* Section PRESERVATION. *)
 
 Variable prog: Seccomp.program.
-Variable tprog: Clight.program.
+Variable tprog: RTL.program.
 Hypothesis TRANSL: Seccompjit.transl_program prog = OK tprog.
 Let ge := Genv.globalenv prog.
 Let tge := Genv.globalenv tprog.
@@ -25,85 +27,110 @@ Proof.
 Qed.
 
 Lemma function_ptr_translated:
-  forall (b: block) (f: fundef),
-  Genv.find_funct_ptr ge b = Some f ->
-  exists tf, Genv.find_funct_ptr tge b = Some tf /\ transl_fundef f = OK tf.
+  forall (b: block) (fd: fundef),
+  Genv.find_funct_ptr ge b = Some fd ->
+  exists tfd, Genv.find_funct_ptr tge b = Some tfd /\ transl_fundef fd = OK tfd.
 Proof.
   exact (Genv.find_funct_ptr_transf_partial _ _ TRANSL).
 Qed.
 
-Lemma sig_translated:
-  forall fd tfd,
-  transl_fundef fd = OK tfd ->
-  Clight.type_of_fundef tfd = Tfunction Tnil type_int32s.
+Lemma functions_translated:
+  forall (v: val) (fd: Seccomp.fundef),
+  Genv.find_funct ge v = Some fd ->
+  exists tfd,
+  Genv.find_funct tge v = Some tfd /\ transl_fundef fd = OK tfd.
 Proof.
-  intros.
-  destruct fd; monadInv H.
-  destruct f; monadInv EQ; auto.
+  exact (Genv.find_funct_transf_partial transl_fundef _ TRANSL).
 Qed.
 
-Inductive match_states: Seccomp.state -> Clight.state -> Prop :=
+Lemma sig_transl_function:
+  forall fd tfd,
+  transl_fundef fd = OK tfd ->
+  RTL.funsig tfd = mksignature nil (Some Tint).
+Proof.
+  intros.
+  destruct fd; monadInv H; auto.
+  monadInv EQ.
+  auto.
+Qed.
+
+Lemma varinfo_preserved:
+  forall b, Genv.find_var_info tge b = Genv.find_var_info ge b.
+Proof.
+  exact (Genv.find_var_info_transf_partial transl_fundef _ TRANSL).
+Qed.
+
+(*
+Inductive match_instr (tc: RTL.code): Seccomp.instruction -> node -> node -> Prop :=
+  | match_Salu_add_k: forall
+      match_instr tc (Salu_add_k k) ns 
+  .
+*)
+
+Inductive match_states: Seccomp.state -> RTL.state -> Prop :=
   | match_state:
-      forall a x sm f pc m tf s k e le tm
+      forall a x sm f pc m tstack tf tsp tpc tregs tm
+        (MA: Vint a = tregs#reg_a)
+        (MX: Vint x = tregs#reg_x)
         (TF: transl_function f = OK tf)
-        (* FIXME: mapping between C statement and seccomp instruction? *)
-        (* FIXME: mapping between a/x/sm and e/le *)
-        (MCONT: k = Kstop)
-        (MEXT: Mem.extends m tm),
+        (MEXT: Mem.extends m tm)
+        (MS: tstack = nil)
+        (MSP: tsp = Vint Int.zero),
       match_states (Seccomp.State a x sm f pc m)
-                   (Clight.State tf s k e le tm)
+                   (RTL.State tstack tf tsp tpc tregs tm)
   | match_callstate:
-      forall fd m tfd args k tm
+      forall fd m tstack tfd targs tm
         (TF: transl_fundef fd = OK tfd)
-        (MCONT: k = Kstop)
-        (MARGS: args = nil)
-        (MEXT: Mem.extends m tm),
+        (MEXT: Mem.extends m tm)
+        (MS: tstack = nil)
+        (MARGS: targs = nil),
       match_states (Seccomp.Callstate fd m)
-                   (Clight.Callstate tfd args k tm)
+                   (RTL.Callstate tstack tfd targs tm)
   | match_returnstate:
-      forall v m tv k tm
+      forall v m tstack tv tm
         (MV: Vint v = tv)
-        (MCONT: k = Kstop)
-        (MEXT: Mem.extends m tm),
+        (MEXT: Mem.extends m tm)
+        (MS: tstack = nil),
       match_states (Seccomp.Returnstate v m)
-                   (Clight.Returnstate tv k tm)
+                   (RTL.Returnstate tstack tv tm)
   .
 
 (*
 Lemma transl_step:
   forall S1 t S2, Seccomp.step ge S1 t S2 ->
   forall R1, match_states S1 R1 ->
-  exists R2, plus Clight.step1 tge R1 t R2 /\ match_states S2 R2.
+  exists R2, plus RTL.step tge R1 t R2 /\ match_states S2 R2.
 *)
 
 Lemma transl_initial_states:
   forall S, Seccomp.initial_state prog S ->
-  exists R, Clight.initial_state tprog R /\ match_states S R.
+  exists R, RTL.initial_state tprog R /\ match_states S R.
 Proof.
-induction 1.
-exploit function_ptr_translated; eauto .
-intros (tf, (A, B)).
-econstructor; split.
- econstructor.
-  apply (Genv.init_mem_transf_partial _ _ TRANSL); eauto .
+  induction 1.
+  exploit function_ptr_translated; eauto.
+  intros (tf, (A, B)).
 
+  econstructor; split.
+
+  (* RTL.initial_state tprog R *)
+  econstructor.
+  apply (Genv.init_mem_transf_partial _ _ TRANSL); eauto.
   rewrite (transform_partial_program_main _ _ TRANSL).
   fold tge.
   rewrite symbols_preserved.
-  eauto .
-
+  eauto.
   eexact A.
-
-  eapply sig_translated.
+  eapply sig_transl_function.
   eexact B.
 
- constructor; auto.
- apply Mem.extends_refl.
+  (* match states S R *)
+  constructor; auto.
+  apply Mem.extends_refl.
 Qed.
 
 Lemma transl_final_states:
   forall S R r,
-  match_states S R -> Seccomp.final_state S r -> Clight.final_state R r.
+  match_states S R -> Seccomp.final_state S r -> RTL.final_state R r.
 Proof.
 intros.
 inv H0.
